src/Lean/Meta/Tactic/Grind/EMatch.lean
@@ -849,7 +849,7 @@ private partial def instantiateTheorem (c : Choice) : M Unit := withDefault do w
     reportEMatchIssue! "unexpected number of parameters at {thm.origin.pp}"
     return ()
   let (some _, c) ← applyAssignment mvars |>.run.run c | return ()
-  let some _ ← synthesizeInsts mvars bis | return ()
+  let some _ ← (synthesizeInsts mvars bis).run | return ()
   if (← checkConstraints thm c.gen proof mvars) then
     let guards ← collectGuards thm proof mvars
     let proof := mkAppN proof mvars
