tests/elab/repr_issue.lean
@@ -14,4 +14,4 @@ foo
 -- The following examples were producing an element of Type `id (Except String Nat)`.
 -- Type class resolution was failing to produce an instance for `Repr (id (Except String Nat))` because `id` is not transparent.
 #eval ex₁.run' (Array.replicate 10 1000) |>.run
-#eval ex₂.run' (Array.replicate 10 1000) |>.run
+#eval ex₂.run.run' (Array.replicate 10 1000) |>.run
